theories/theories/utp_reactive.thy
@@ -15,8 +15,8 @@ begin
 default_sort REACTIVE_SORT
 
 abbreviation "wait \<equiv> MkPlainP ''wait'' True TYPE(bool) TYPE('m)"
-abbreviation "tr   \<equiv> MkPlainP ''tr'' True TYPE('m EVENT list) TYPE('m)"
-abbreviation "ref  \<equiv> MkPlainP ''ref'' True TYPE('m EVENT fset) TYPE('m)"
+abbreviation "tr   \<equiv> MkPlainP ''tr'' True TYPE('m EVENT ULIST) TYPE('m)"
+abbreviation "ref  \<equiv> MkPlainP ''ref'' True TYPE('m EVENT UFSET) TYPE('m)"
 
 definition SkipREA :: "'a WF_PREDICATE" where
 "SkipREA = `(\<not> ok \<and> ($tr \<le> $tr\<acute>)) \<or> (ok\<acute> \<and> II\<^bsub>REL_VAR - OKAY\<^esub>)`"
@@ -32,15 +32,15 @@ declare SkipREA_def [eval, evalr]
 text {* R1 ensures that the trace only gets longer *}
 
 definition R1 :: " 'a WF_PREDICATE \<Rightarrow> 'a WF_PREDICATE" where
-"R1 P = `P \<and> ($tr \<le> $tr\<acute>)`"
+"R1(P) = `P \<and> ($tr \<le> $tr\<acute>)`"
 
 text {* R2 ensures that the trace only gets longer *}
 
 definition R2 :: "'a WF_PREDICATE \<Rightarrow> 'a WF_PREDICATE" where
-"R2 P = `P[\<langle>\<rangle> / tr]\<^sub>*[($tr\<acute> - $tr) / tr\<acute>]\<^sub>*`"
+"R2(P) = `P[\<langle>\<rangle> / tr][($tr\<acute> - $tr) / tr\<acute>]`"
 
 definition R3 :: "'a WF_PREDICATE \<Rightarrow> 'a WF_PREDICATE" where
-"R3 P = `II\<^bsub>rea\<^esub> \<lhd> $[wait]\<^sub>* \<rhd> P`"
+"R3(P) = `II\<^bsub>rea\<^esub> \<lhd> $wait \<rhd> P`"
 
 definition R :: "'a WF_PREDICATE \<Rightarrow> 'a WF_PREDICATE" where 
 "R P = (R1 \<circ> R2 \<circ> R3)P"
@@ -57,31 +57,72 @@ translations
   "_upred_R3 P" == "CONST R3 P"
   "_upred_R P" == "CONST R P"
 
+lemma PVAR_VAR_inj [dest]:
+  fixes x y :: "('a :: DEFINED, 'm :: VALUE) PVAR"
+  assumes "x\<down> = y\<down>"
+  shows "x = y"
+   by (metis PVAR_VAR_inv assms)
+
+lemma PSubstPE_PVarPE_neq [usubst]:
+  fixes v :: "('a :: DEFINED, 'm :: VALUE) WF_PEXPRESSION"
+  and   x :: "('b :: DEFINED, 'm :: VALUE) PVAR"
+  assumes "TYPEUSOUND('a, 'm)" "x\<down> \<noteq> y\<down>" "v \<rhd>\<^sub>* y"
+  shows "PSubstPE (PVarPE x) v y = PVarPE x"
+  using assms by (auto simp add:eval typing defined pevar_compat_def)
+
+lemma var_name_uniq [simp]: 
+  "name x \<noteq> name y \<Longrightarrow> x \<noteq> y"
+  by (auto)
+
+lemma name_str_uniq [simp]: 
+  "name_str x \<noteq> name_str y \<Longrightarrow> x \<noteq> y"
+  by (auto)
+
+declare EvalPE_PSubstPE [evalp]
+
+lemma SubstP_PSubstPE [usubst]:
+  fixes v :: "('a :: DEFINED, 'm :: VALUE) WF_PEXPRESSION"
+  and   e :: "('b :: DEFINED, 'm :: VALUE) WF_PEXPRESSION"
+  assumes "TYPEUSOUND('a, 'm)" "TYPEUSOUND('b, 'm)" "v \<rhd>\<^sub>* x"
+  shows "e\<down>[v\<down>/\<^sub>ex\<down>] = (PSubstPE e v x)\<down>"
+  using assms by (auto simp add:evale typing defined evalp)
+
+term "(PVarPE x)"
+
+lemma PVarPE_VarP [simp]:
+  fixes x :: "(bool, 'm::BOOL_SORT) PVAR"
+  shows "((PVarPE x)\<down> ==\<^sub>p (TruePE\<down>)) = VarP (x\<down>)"
+  apply (utp_pred_auto_tac)
+  apply (metis BOOL_SORT_class.Inverse)
+done
+
 
 lemma SkipREA_CondR_SkipR: 
   "`II\<^bsub>rea\<^esub>` = `II \<lhd> ok \<rhd> ($tr \<le> $tr\<acute>)`"
 proof -
 
   have "`II \<lhd> ok \<rhd> ($tr \<le> $tr\<acute>)` = `($okay\<acute> = $okay \<and> II\<^bsub>REL_VAR - OKAY\<^esub>) \<lhd> ok \<rhd> ($tr \<le> $tr\<acute>)`"
-    by (metis Diff_cancel ExistsP_empty HOMOGENEOUS_REL_VAR MkPlain_UNDASHED SkipRA.rep_eq SkipRA_unfold UnCI hom_alphabet_undash)
+    by (simp add:SkipR_as_SkipRA SkipRA_unfold[of "okay\<down>"] closure erasure typing)
 
-  also have "... = `($okay\<acute> = $okay \<and> II\<^bsub>REL_VAR - OKAY\<^esub>)[true/okay] \<lhd> $okay \<rhd> (($tr \<le> $tr\<acute>)[false/okay])`"
-    by (rule CondR_VarP_aux, simp_all add:typing defined)
+  also 
+  have "... = `($okay\<acute> = $okay \<and> II\<^bsub>REL_VAR - OKAY\<^esub>)[true/okay] 
+               \<lhd> ok \<rhd> 
+               (($tr \<le> $tr\<acute>)[false/okay])`"
+    by (simp add:erasure, rule_tac CondR_VarP_aux[of "okay\<down>"], simp_all)
 
-  also have "... = `(ok \<and> II\<^bsub>REL_VAR - OKAY\<^esub>) \<lhd> ok \<rhd> ($tr \<le> $tr\<acute>)`"
-  proof -
-(*
-    have "(ulesseq :: 'b \<Rightarrow> 'b \<Rightarrow> 'b) \<in> FUNC2 (ListType StringType) (ListType StringType) BoolType"
-      by (simp add: closure) 
+  also have "... = `(ok' \<and> II\<^bsub>REL_VAR - OKAY\<^esub>) \<lhd> ok \<rhd> ($tr \<le> $tr\<acute>)`"
+    by (simp add:usubst typing defined closure)
 
-    thus ?thesis
+  also have "... = `(ok \<and> ok' \<and> II\<^bsub>REL_VAR - OKAY\<^esub>) \<or> (\<not> ok \<and> ($tr \<le> $tr\<acute>))`"
+    by (utp_pred_auto_tac)
 
-      apply (insert SubstE_Op2E[of "VarE tr :: 'b WF_EXPRESSION" "ListType StringType" "VarE tr\<acute>" "ListType StringType" "ulesseq" BoolType "FalseE" "okay"])
+  also have "... = `II\<^bsub>rea\<^esub>`"
+    apply (simp add:SkipREA_def)
+    apply (rule_tac x="okay\<down>" in BoolType_aux_var_split_eq_intro)
+    apply (simp_all add:usubst closure typing defined)
+  sorry
 
-    apply (simp add:usubst typing defined closure var_simps)
-*)
-
-  oops (* FIXME: Can't finish the step without more laws about prefix *)
-
+  finally show ?thesis ..
+qed
 
 end
