theories/types/utp_fset.thy
@@ -1,0 +1,33 @@
+(******************************************************************************)
+(* Project: Unifying Theories of Programming in HOL                           *)
+(* File: utp_fset.thy                                                         *)
+(* Author: Simon Foster, University of York (UK)                              *)
+(******************************************************************************)
+
+header {* UTP Finite Sets *}
+
+theory utp_fset
+imports 
+  "../core/utp_value"
+  "../core/utp_sorts"
+  "../core/utp_event"
+  "../tactics/utp_pred_tac"
+  "../tactics/utp_expr_tac"
+begin
+
+typedef 'a::DEFINED UFSET = "{xs :: 'a fset. \<forall>x\<in>\<^sub>fxs. \<D> x}"
+  apply (rule_tac x="\<lbrace>\<rbrace>" in exI)
+  apply (auto)
+done
+
+instantiation UFSET :: (DEFINED) DEFINED
+begin
+definition "Defined_UFSET (xs :: 'a UFSET) = True"
+instance ..
+end
+
+lemma Defined_UFSET [defined]: 
+  "\<D> (xs :: ('a::DEFINED UFSET))"
+  by (simp add:Defined_UFSET_def)
+
+end
